BinaryHeap/CompleteTree/AdditionalProofs/Contains.lean
@@ -3,93 +3,46 @@ import BinaryHeap.CompleteTree.AdditionalProofs.Get
 
 namespace BinaryHeap.CompleteTree.AdditionalProofs
 
-private theorem if_get_eq_contains {α : Type u} {o : Nat} (tree : CompleteTree α (o+1)) (element : α) (index : Fin (o+1)) : tree.get' index = element → tree.contains element := by
-    unfold get' contains
-    simp only [Nat.succ_eq_add_one, Fin.zero_eta, Nat.add_eq, ne_eq]
-    split
-    case h_1 p q v l r _ _ _ _ =>
-      intro h₁
-      split; omega
-      rename α => vv
-      rename_i hsum heq
-      have h₂ := heqSameRoot (hsum) (Nat.succ_pos (p+q)) heq
-      rw[root_unfold] at h₂
-      rw[root_unfold] at h₂
-      simp only [←h₂, h₁, true_or]
-    case h_2 index p q v l r _ _ _ _ h₃ =>
-      intro h₄
-      split ; rename_i hx _; exact absurd hx (Nat.succ_ne_zero _)
-      case h_2 pp qq vv ll rr _ _  _ h₅ heq =>
-      have : p = pp := heqSameLeftLen h₅ (Nat.succ_pos _) heq
-      have : q = qq := heqSameRightLen h₅ (Nat.succ_pos _) heq
-      subst pp qq
-      simp only [Nat.add_eq, Nat.succ_eq_add_one, heq_eq_eq, branch.injEq] at heq
-      have : v = vv := heq.left
-      have : l = ll := heq.right.left
-      have : r = rr := heq.right.right
-      subst vv ll rr
-      revert h₄
-      split
-      all_goals
-        split
-        intro h₄
-        right
+private theorem if_get_eq_contains {α : Type u} {n : Nat} (tree : CompleteTree α n) (element : α) (index : Fin n) : tree.get index = element → tree.contains element := by
+    rw[get_unfold]
+    rw[contains_as_root_left_right]
+    intro h₁
+    split at h₁
+    case isTrue =>
+      left
+      assumption
+    case isFalse h =>
+      have _termination : index.val ≠ 0 := Fin.val_ne_iff.mpr h
+      right
+      simp only at h₁
+      split at h₁
       case' isTrue => left
       case' isFalse => right
       all_goals
-        revert h₄
+        revert h₁
         apply if_get_eq_contains
-        done
+termination_by index.val
 
-private theorem if_contains_get_eq_auxl {α : Type u} {o : Nat} (tree : CompleteTree α (o+1)) (element : α) :
-  ∀(indexl : Fin (tree.leftLen (Nat.succ_pos o))), (tree.left _).get indexl = element → ∃(index : Fin (o+1)), tree.get index = element
+private theorem if_contains_get_eq_auxl {α : Type u} {n : Nat} (tree : CompleteTree α n) (element : α) (h₁ : n > 0):
+  ∀(indexl : Fin (tree.leftLen h₁)), (tree.left _).get indexl = element → ∃(index : Fin n), tree.get index = element
 := by
   intro indexl
-  let index : Fin (o+1) := indexl.succ.castLT (by
-    simp only [Nat.succ_eq_add_one, Fin.val_succ, Nat.succ_lt_succ_iff, gt_iff_lt]
-    exact Nat.lt_of_lt_of_le indexl.isLt $ Nat.le_of_lt_succ $ leftLenLtN tree (Nat.succ_pos o)
-  )
+  let index : Fin n := indexl.succ.castLT (Nat.lt_of_le_of_lt (Nat.succ_le_of_lt indexl.isLt) (leftLenLtN tree h₁))
   intro prereq
   exists index
-  unfold get
-  simp
-  unfold get'
-  generalize hindex : index = i
-  split
-  case h_1 =>
-    have : index.val = 0 := Fin.val_eq_of_eq hindex
-    contradiction
-  case h_2 j p q v l r ht1 ht2 ht3 _ _ =>
-    have h₂ : index.val = indexl.val + 1 := rfl
-    have h₃ : index.val = j.succ := Fin.val_eq_of_eq hindex
-    have h₄ : j = indexl.val := Nat.succ.inj $ h₃.subst (motive := λx↦ x = indexl.val + 1) h₂
-    have : p = (branch v l r ht1 ht2 ht3).leftLen (Nat.succ_pos _) := rfl
-    have h₅ : j < p := by simp only [this, indexl.isLt, h₄]
-    simp only [h₅, ↓reduceDIte, Nat.add_eq]
-    unfold get at prereq
-    split at prereq
-    rename_i pp ii ll hel hei heq
-    split
-    rename_i ppp lll _ _ _ _ _ _
-    have : pp = ppp := by omega
-    subst pp
-    simp only [gt_iff_lt, Nat.succ_eq_add_one, Nat.add_eq, heq_eq_eq, Nat.zero_lt_succ] at *
-    have : j = ii.val := by omega
-    subst j
-    simp
-    rw[←hei] at prereq
-    rw[left_unfold] at heq
-    rw[heq]
-    assumption
+  have h₂ : index > ⟨0,h₁⟩ := Nat.zero_lt_of_ne_zero $ Fin.val_ne_iff.mpr $ Fin.succ_ne_zero _
+  have h₃ : index.val ≤ tree.leftLen h₁ := Nat.succ_le_of_lt indexl.isLt
+  rw[get_left _ _ h₂ h₃]
+  exact prereq
 
-private theorem if_contains_get_eq_auxr {α : Type u} {o : Nat} (tree : CompleteTree α (o+1)) (element : α) :
-  ∀(indexl : Fin (tree.rightLen (Nat.succ_pos o))), (tree.right _).get indexl = element → ∃(index : Fin (o+1)), tree.get index = element
+private theorem if_contains_get_eq_auxr {α : Type u} {n : Nat} (tree : CompleteTree α n) (element : α) (h₁ : n > 0):
+  ∀(indexr : Fin (tree.rightLen h₁)), (tree.right _).get indexr = element → ∃(index : Fin n), tree.get index = element
 := by
   intro indexr
-  let index : Fin (o+1) := ⟨(tree.leftLen (Nat.succ_pos o) + indexr.val + 1), by
-    have h₂ : tree.leftLen (Nat.succ_pos _) + tree.rightLen _ + 1 = tree.length := Eq.symm $ lengthEqLeftRightLenSucc tree _
+  let index : Fin n := ⟨(tree.leftLen h₁ + indexr.val + 1), by
+    have h₂ : tree.leftLen h₁ + tree.rightLen _ + 1 = tree.length := Eq.symm $ lengthEqLeftRightLenSucc tree _
     rw[length] at h₂
-    have h₃ : tree.leftLen (Nat.succ_pos o) + indexr.val + 1 < tree.leftLen (Nat.succ_pos o) + tree.rightLen (Nat.succ_pos o) + 1 := by
+    have h₃ : tree.leftLen h₁ + indexr.val + 1 < tree.leftLen h₁ + tree.rightLen h₁ + 1 := by
       apply Nat.succ_lt_succ
       apply Nat.add_lt_add_left
       exact indexr.isLt
@@ -97,95 +50,39 @@ private theorem if_contains_get_eq_auxr {α : Type u} {o : Nat} (tree : Complete
   ⟩
   intro prereq
   exists index
-  unfold get
-  simp
-  unfold get'
-  generalize hindex : index = i
-  split
-  case h_1 =>
-    have : index.val = 0 := Fin.val_eq_of_eq hindex
-    contradiction
-  case h_2 j p q v l r ht1 ht2 ht3 _ _ =>
-    have h₂ : index.val = (branch v l r ht1 ht2 ht3).leftLen (Nat.succ_pos _) + indexr.val + 1 := rfl
-    have h₃ : index.val = j.succ := Fin.val_eq_of_eq hindex
-    have h₄ : j = (branch v l r ht1 ht2 ht3).leftLen (Nat.succ_pos _) + indexr.val := by
-      rw[h₃] at h₂
-      exact Nat.succ.inj h₂
-    have : p = (branch v l r ht1 ht2 ht3).leftLen (Nat.succ_pos _) := rfl
-    have h₅ : ¬(j < p) := by simp_arith [this, h₄]
-    simp only [h₅, ↓reduceDIte, Nat.add_eq]
-    unfold get at prereq
-    split at prereq
-    rename_i pp ii rr hel hei heq
-    split
-    rename_i ppp rrr _ _ _ _ _ _ _
-    have : pp = ppp := by rw[rightLen_unfold] at hel; exact Nat.succ.inj hel.symm
-    subst pp
-    simp only [gt_iff_lt, ne_eq, Nat.succ_eq_add_one, Nat.add_eq, Nat.reduceEqDiff, heq_eq_eq, Nat.zero_lt_succ] at *
-    have : j = ii.val + p := by omega
-    subst this
-    simp
-    rw[right_unfold] at heq
-    rw[heq]
-    assumption
+  have h₂ : tree.leftLen h₁ < tree.leftLen h₁ + indexr.val + 1 := Nat.lt_of_le_of_lt (Nat.le_add_right _ _) (Nat.lt_succ_self _)
+  rw[get_right _ index h₂]
+  have : index.val - tree.leftLen h₁ - 1 = indexr.val :=
+    have : index.val = tree.leftLen h₁ + indexr.val + 1 := rfl
+    have : index.val = indexr.val + tree.leftLen h₁ + 1 := (Nat.add_comm indexr.val (tree.leftLen h₁)).substr this
+    have : index.val - (tree.leftLen h₁ + 1) = indexr.val := Nat.sub_eq_of_eq_add this
+    (Nat.sub_sub _ _ _).substr this
+  simp only[this]
+  assumption
 
-private theorem if_contains_get_eq {α : Type u} {o : Nat} (tree : CompleteTree α (o+1)) (element : α) (h₁ : tree.contains element) : ∃(index : Fin (o+1)), tree.get' index = element := by
-    revert h₁
-    unfold contains
-    split ; rename_i hx _; exact absurd hx (Nat.succ_ne_zero o)
-    rename_i n m v l r _ _ _ he heq
-    intro h₁
+private theorem if_contains_get_eq {α : Type u} {n : Nat} (tree : CompleteTree α n) (element : α) (h₁ : tree.contains element) : ∃(index : Fin n), tree.get index = element := by
+    unfold contains at h₁
+    match n, tree with
+    | 0, .leaf => contradiction
+    | (o+p+1), .branch v l r o_le_p max_height_diff subtree_complete =>
     cases h₁
-    case h_2.inl h₂ =>
-      unfold get'
+    case inl h₂ =>
       exists 0
-      split
-      case h_2 hx => have hx := Fin.val_eq_of_eq hx; simp at hx;
-      case h_1 vv _ _ _ _ _ _ _ =>
-        have h₃ := heqSameRoot he (Nat.succ_pos _) heq
-        simp only[root_unfold] at h₃
-        simp only[h₃, h₂]
-    rename_i h
-    cases h
-    case h_2.inr.inl h₂ => exact
-      match hn : n, hl: l with
-      | 0, .leaf => by contradiction
-      | (nn+1), l => by
-        have nn_lt_o : nn < o := by have : o = nn + 1 + m := Nat.succ.inj he; omega --also for termination
-        have h₃ := if_contains_get_eq l element h₂
-        have h₄ := if_contains_get_eq_auxl tree element
-        simp only at h₄
-        simp[get_eq_get'] at h₃ ⊢
-        apply h₃.elim
-        match o, tree with
-        | (yy+_), .branch _ ll _ _ _ _ =>
-          simp_all[left_unfold, leftLen_unfold]
-          have : yy = nn+1 := heqSameLeftLen (by omega) (Nat.succ_pos _) heq
-          have : _ = m := heqSameRightLen (by omega) (Nat.succ_pos _) heq
-          subst yy m
-          simp_all
-          exact h₄
-    case h_2.inr.inr h₂ => exact
-      match hm : m, hr: r with
-      | 0, .leaf => by contradiction
-      | (mm+1), r => by
-        have mm_lt_o : mm < o := by have : o = n + (mm + 1) := Nat.succ.inj he; omega --termination
-        have h₃ := if_contains_get_eq r element h₂
-        have h₄ := if_contains_get_eq_auxr tree element
-        simp[get_eq_get'] at h₃ ⊢
-        apply h₃.elim
-        match o, tree with
-        | (_+zz), .branch _ _ rr _ _ _ =>
-          simp_all[right_unfold, rightLen_unfold]
-          have : _ = n := heqSameLeftLen (by omega) (Nat.succ_pos _) heq
-          have : zz = mm+1 := heqSameRightLen (by omega) (Nat.succ_pos _) heq
-          subst n zz
-          simp_all
-          exact h₄
-  termination_by o
+    case inr h₂ =>
+      cases h₂
+      case inl h₂ =>
+        have h₄ := if_contains_get_eq l element h₂
+        have h₅ := if_contains_get_eq_auxl (.branch v l r o_le_p max_height_diff subtree_complete) element (Nat.succ_pos _)
+        apply h₄.elim
+        assumption
+      case inr h₂ =>
+        have h₄ := if_contains_get_eq r element h₂
+        have h₅ := if_contains_get_eq_auxr (.branch v l r o_le_p max_height_diff subtree_complete) element (Nat.succ_pos _)
+        apply h₄.elim
+        assumption
 
 
-theorem contains_iff_index_exists' {α : Type u} {o : Nat} (tree : CompleteTree α (o+1)) (element : α) : tree.contains element ↔ ∃ (index : Fin (o+1)), tree.get' index = element := by
+theorem contains_iff_index_exists' {α : Type u} {n : Nat} (tree : CompleteTree α n) (element : α) : tree.contains element ↔ ∃ (index : Fin n), tree.get index = element := by
   constructor
   case mpr =>
     simp only [forall_exists_index]
