BinaryHeap/CompleteTree/AdditionalProofs/Get.lean
@@ -3,64 +3,39 @@ import BinaryHeap.CompleteTree.Lemmas
 
 namespace BinaryHeap.CompleteTree.AdditionalProofs
 
-theorem get_eq_get' {α : Type u} {n : Nat} (tree : CompleteTree α (n+1)) (index : Fin (n+1)) : tree.get' index = tree.get index := rfl
+theorem get_zero_eq_root {α : Type u} {n : Nat} (tree : CompleteTree α n) (h₁ : n > 0): tree.root h₁ = tree.get ⟨0,h₁⟩ :=
+  match h₂ : n, h₃ : (⟨0,h₁⟩ : Fin n), tree with
+  | (_+_+1), 0, .branch v _ _ _ _ _ => rfl
+  | nn+1, ⟨j+1,h₄⟩, _ => by
+    subst h₂
+    simp only [heq_eq_eq, Fin.ext_iff] at h₃
 
-theorem get_zero_eq_root {α : Type u} {n : Nat} (tree : CompleteTree α n) (h₁ : n > 0): tree.root h₁ = tree.get ⟨0,h₁⟩ := by
-  unfold get
-  match n with
-  | nn+1 =>
-    unfold get'
-    split
-    case h_2 hx => exact absurd (Fin.mk.inj hx) (Nat.zero_ne_add_one _)
-    case h_1 => trivial
-
-theorem get_right {α : Type u} {n : Nat} (tree : CompleteTree α n) (index : Fin n) (h₁ : n > 0) (h₂ : index > tree.leftLen h₁) :
-  have h₃ : ↑index - tree.leftLen h₁ - 1 < tree.rightLen h₁ := by
-    revert h₂
-    unfold leftLen rightLen length
-    split
-    intro h₂
-    rename_i o p v l r _ _ _ _
-    have h₃ := index.isLt
-    apply Nat.sub_lt_right_of_lt_add
-    omega
-    apply Nat.sub_lt_right_of_lt_add
-    omega
-    have : p+1+o = (o.add p).succ := by simp_arith
-    rw[this]
-    assumption
-  tree.get index = (tree.right h₁).get ⟨index.val - (tree.leftLen h₁) - 1, h₃⟩
-:=
-  match n, tree with
-  | (o+p+1), .branch v l r _ _ _ => by
-    simp[right_unfold, leftLen_unfold]
-    rw[leftLen_unfold] at h₂
-    generalize hnew : get ⟨↑index - o - 1, _⟩ r = new
-    unfold get get'
-    split
-    case h_1 =>
-      contradiction
-    case h_2 j h₃ o2 p2 v2 l2 r2 _ _ _ d1 he₁ he₂ _ =>
-      clear d1
-      have : o = o2 := heqSameLeftLen (congrArg Nat.succ he₁) (Nat.succ_pos _) he₂
-      have : p = p2 := heqSameRightLen (congrArg Nat.succ he₁) (Nat.succ_pos _) he₂
-      subst o2 p2
-      simp at he₂
-      have : v = v2 := he₂.left
-      have : l = l2 := he₂.right.left
-      have : r = r2 := he₂.right.right
-      subst r2 l2 v2
-      simp_all
-      have : ¬j < o := by simp_arith[h₂]
-      simp[this]
-      cases p <;> simp
-      case zero =>
-        omega
-      case succ pp _ _ _ _ _ _ =>
-        have : j + 1 - o - 1 = j - o := by omega
-        simp[this] at hnew
-        rw[get_eq_get']
-        assumption
+theorem get_right {α : Type u} {n : Nat} (tree : CompleteTree α n) (index : Fin n) (h₂ : index > tree.leftLen (Nat.zero_lt_of_lt index.isLt))
+  : have h₁ : n > 0 := Nat.zero_lt_of_lt index.isLt
+    have h₃ : ↑index - tree.leftLen h₁ - 1 < tree.rightLen h₁ := by
+      revert h₂
+      unfold leftLen rightLen length
+      split
+      intro h₂
+      rename_i o p v l r _ _ _
+      have h₃ := index.isLt
+      apply Nat.sub_lt_right_of_lt_add
+      omega
+      apply Nat.sub_lt_right_of_lt_add
+      omega
+      have : p+1+o = (o.add p).succ := by simp_arith
+      rw[this]
+      assumption
+    tree.get index = (tree.right h₁).get ⟨index.val - (tree.leftLen h₁) - 1, h₃⟩
+  :=
+  match n, index, tree with
+  | (o+p+1), ⟨j+1,h₃⟩, .branch _ _ r _ _ _ =>
+    if h₄ : j < o then
+      absurd h₄ $ Nat.not_lt_of_ge (Nat.le_of_lt_succ h₂)
+    else by
+      simp only[right_unfold, leftLen_unfold]
+      have : j + 1 - o - 1 = j - o := by omega
+      simp (config := {autoUnfold := true})[this, h₄]
 
 theorem get_right' {α : Type u} {n m : Nat} {v : α} {l : CompleteTree α n} {r : CompleteTree α m} {m_le_n : m ≤ n} {max_height_diff : n < 2 * (m + 1)} {subtree_complete : (n + 1).isPowerOfTwo ∨ (m + 1).isPowerOfTwo} (index : Fin (n + m + 1)) (h₁ : index > n) :
   have h₂ : ↑index - n - 1 < m := by
@@ -74,36 +49,73 @@ theorem get_right' {α : Type u} {n m : Nat} {v : α} {l : CompleteTree α n} {r
     assumption
   (branch v l r m_le_n max_height_diff subtree_complete).get index = r.get ⟨index.val - n - 1, h₂⟩
 :=
-  get_right (branch v l r m_le_n max_height_diff subtree_complete) index (Nat.succ_pos _) h₁
+  get_right (branch v l r m_le_n max_height_diff subtree_complete) index h₁
 
-theorem get_left {α : Type u} {n : Nat} (tree : CompleteTree α n) (index : Fin n) (h₁ : n > 0) (h₂ : index > ⟨0, h₁⟩) (h₃ : index ≤ tree.leftLen h₁) :
+theorem get_left {α : Type u} {n : Nat} (tree : CompleteTree α n) (index : Fin n) (h₂ : index > ⟨0, (Nat.zero_lt_of_lt index.isLt)⟩) (h₃ : index ≤ tree.leftLen (Nat.zero_lt_of_lt index.isLt)) :
+  have h₁ : n > 0 := Nat.zero_lt_of_lt index.isLt
   have h₃ : ↑index - 1 < tree.leftLen h₁ := Nat.lt_of_lt_of_le (Nat.pred_lt_self h₂) h₃
   tree.get index = (tree.left h₁).get ⟨index.val - 1, h₃⟩
 :=
-  match n, tree with
-  | (o+p+1), .branch v l r _ _ _ => by
-    simp[left_unfold]
-    generalize hnew : get ⟨↑index - 1, _⟩ l = new
-    unfold get get'
-    split
-    case h_1 => contradiction
-    case h_2 j h₃ o2 p2 v2 l2 r2 _ _ _ d1 he₁ he₂ =>
-      clear d1
-      have : o = o2 := heqSameLeftLen (congrArg Nat.succ he₁) (Nat.succ_pos _) he₂
-      have : p = p2 := heqSameRightLen (congrArg Nat.succ he₁) (Nat.succ_pos _) he₂
-      subst o2 p2
-      simp[leftLen_unfold] at h₃
-      have h₄ : j < o :=Nat.lt_of_succ_le h₃
-      simp[h₄]
-      cases o ; contradiction
-      case succ oo =>
-        simp at hnew he₂ ⊢
-        have := he₂.right.left
-        subst l2
-        assumption
+    match n, index, tree with
+  | (o+p+1), ⟨j+1,h₅⟩, .branch _ l _ _ _ _ =>
+    if h₄ : j < o then by
+      simp only[left_unfold, leftLen_unfold]
+      have : j + 1 - o - 1 = j - o := by omega
+      simp (config := {autoUnfold := true})[this, h₄]
+    else
+      absurd (Nat.lt_of_succ_le h₃) h₄
 
 theorem get_left' {α : Type u} {n m : Nat} {v : α} {l : CompleteTree α n} {r : CompleteTree α m} {m_le_n : m ≤ n} {max_height_diff : n < 2 * (m + 1)} {subtree_complete : (n + 1).isPowerOfTwo ∨ (m + 1).isPowerOfTwo} (index : Fin (n + m + 1)) (h₁ : index > ⟨0, Nat.succ_pos _⟩) (h₂ : index ≤ n) :
   have h₃ : ↑index - 1 < n := Nat.lt_of_lt_of_le (Nat.pred_lt_self h₁) h₂
   (branch v l r m_le_n max_height_diff subtree_complete).get index = l.get ⟨index.val - 1, h₃⟩
 :=
-  get_left (branch v l r m_le_n max_height_diff subtree_complete) index (Nat.succ_pos _) h₁ h₂
+  get_left (branch v l r m_le_n max_height_diff subtree_complete) index h₁ h₂
+
+theorem get_unfold {α : Type u} {n : Nat} (tree : CompleteTree α n) (index : Fin n)
+  :
+  have h₁ : n > 0 := (Nat.zero_lt_of_lt index.isLt)
+  tree.get index =
+    if h₂ : index = ⟨0, h₁⟩ then
+      tree.root h₁
+    else if h₃ : index ≤ tree.leftLen h₁ then
+      have h₃ : ↑index - 1 < tree.leftLen h₁ := Nat.lt_of_lt_of_le (Nat.pred_lt_self $ Nat.zero_lt_of_ne_zero $ Fin.val_ne_iff.mpr h₂) h₃
+      (tree.left h₁).get ⟨index.val - 1, h₃⟩
+    else
+      have h₃ : ↑index - tree.leftLen h₁ - 1 < tree.rightLen h₁ := by
+        revert h₃
+        unfold leftLen rightLen length
+        split
+        intro h₂
+        rename_i o p v l r _ _ _ _ _
+        have h₃ := index.isLt
+        apply Nat.sub_lt_right_of_lt_add
+        omega
+        apply Nat.sub_lt_right_of_lt_add
+        omega
+        have : p+1+o = (o.add p).succ := by simp_arith
+        rw[this]
+        assumption
+      (tree.right h₁).get ⟨index.val - (tree.leftLen h₁) - 1, h₃⟩
+  :=
+  have h₁ : n > 0 := (Nat.zero_lt_of_lt index.isLt)
+  if h₂ : index = ⟨0, h₁⟩ then by
+    simp only [h₂]
+    exact Eq.symm $ get_zero_eq_root _ _
+  else if h₃ : index ≤ tree.leftLen h₁ then by
+    simp [h₂, h₃]
+    exact get_left tree index (Nat.zero_lt_of_ne_zero $ Fin.val_ne_iff.mpr h₂) h₃
+  else by
+    simp [h₂, h₃]
+    exact get_right tree index (Nat.gt_of_not_le h₃)
+
+theorem get_unfold' {α : Type u} {n m : Nat} {v : α} {l : CompleteTree α n} {r : CompleteTree α m} {m_le_n : m ≤ n} {max_height_diff : n < 2 * (m + 1)} {subtree_complete : (n + 1).isPowerOfTwo ∨ (m + 1).isPowerOfTwo} (index : Fin (n + m + 1)) :
+  (branch v l r m_le_n max_height_diff subtree_complete).get index = if h₂ : index = ⟨0, Nat.zero_lt_of_lt index.isLt⟩ then
+      v
+    else if h₃ : index ≤ n then
+      have h₃ : ↑index - 1 < n := Nat.lt_of_lt_of_le (Nat.pred_lt_self $ Nat.zero_lt_of_ne_zero $ Fin.val_ne_iff.mpr h₂) h₃
+      l.get ⟨index.val - 1, h₃⟩
+    else
+      have h₃ : ↑index - n - 1 < m := by omega
+      r.get ⟨index.val - n - 1, h₃⟩
+  :=
+    get_unfold _ _
