BinaryHeap/CompleteTree/AdditionalProofs/HeapRemoveLast.lean
@@ -7,84 +7,39 @@ import BinaryHeap.CompleteTree.NatLemmas
 namespace BinaryHeap.CompleteTree.AdditionalProofs
 
 /--Shows that the index and value returned by heapRemoveLastWithIndex are consistent.-/
-protected theorem heapRemoveLastWithIndexReturnsItemAtIndex {α : Type u} {o : Nat} (heap : CompleteTree α (o+1)) : heap.get' (Internal.heapRemoveLastWithIndex heap).snd.snd = (Internal.heapRemoveLastWithIndex heap).snd.fst := by
+protected theorem heapRemoveLastWithIndexReturnsItemAtIndex {α : Type u} {o : Nat} (heap : CompleteTree α (o+1)) : heap.get (Internal.heapRemoveLastWithIndex heap).snd.snd = (Internal.heapRemoveLastWithIndex heap).snd.fst := by
   unfold CompleteTree.Internal.heapRemoveLastWithIndex CompleteTree.Internal.heapRemoveLastAux
   split
   rename_i n m v l r m_le_n max_height_difference subtree_full
   simp only [Nat.add_eq, Fin.zero_eta, Fin.isValue, decide_eq_true_eq, Fin.castLE_succ]
   split
   case isTrue n_m_zero =>
-    unfold get'
-    split
-    case h_1 nn mm vv ll rr mm_le_nn _ _ _ _ he₁ he₂ =>
-      have h₁ : n = 0 := And.left $ Nat.add_eq_zero.mp n_m_zero.symm
-      have h₂ : m = 0 := And.right $ Nat.add_eq_zero.mp n_m_zero.symm
-      have h₃ : nn = 0 := And.left (Nat.add_eq_zero.mp $ Eq.symm $ (Nat.zero_add 0).subst (motive := λx ↦ x = nn + mm) $ h₂.subst (motive := λx ↦ 0 + x = nn + mm) (h₁.subst (motive := λx ↦ x + m = nn + mm) he₁))
-      have h₄ : mm = 0 := And.right (Nat.add_eq_zero.mp $ Eq.symm $ (Nat.zero_add 0).subst (motive := λx ↦ x = nn + mm) $ h₂.subst (motive := λx ↦ 0 + x = nn + mm) (h₁.subst (motive := λx ↦ x + m = nn + mm) he₁))
-      subst n m nn mm
-      exact And.left $ CompleteTree.branch.inj (eq_of_heq he₂.symm)
-    case h_2 =>
-      omega -- to annoying to deal with Fin.ofNat... There's a hypothesis that says 0 = ⟨1,_⟩.
+    have h₁ : n = 0 := And.left $ Nat.add_eq_zero.mp n_m_zero.symm
+    have h₂ : m = 0 := And.right $ Nat.add_eq_zero.mp n_m_zero.symm
+    subst n m
+    rfl
   case isFalse n_m_not_zero =>
-    unfold get'
     split
-    case h_1 nn mm vv ll rr mm_le_nn max_height_difference_2 subtree_full2 _ he₁ he₂ he₃ =>
-      --aaaaaaaaaaaaaaaaaaaaaaaaaaaaaa
-      --okay, I know that he₁ is False.
-      --but reducing this wall of text to something the computer understands - I am frightened.
-      exfalso
-      revert he₁
-      split
-      case' isTrue => cases l; case leaf hx => exact absurd hx.left $ Nat.not_lt_zero m
-      all_goals
-        apply Fin.ne_of_val_ne
-        simp only [Fin.isValue, Fin.val_succ, Fin.coe_castLE, Fin.coe_addNat, Nat.add_one_ne_zero, not_false_eq_true]
-      --okay, this wasn't that bad
-    case h_2 j j_lt_n_add_m nn mm vv ll rr mm_le_nn max_height_difference_2 subtree_full2 heap he₁ he₂ he₃ =>
-      --he₁ relates j to the other indices. This is the important thing here.
-      --it should be reducible to j = (l or r).heap.heapRemoveLastWithIndex.snd.snd
-      --or something like it.
-
-      --but first, let's get rid of mm and nn, and vv while at it.
-      -- which are equal to m, n, v, but we need to deduce this from he₃...
-      have : n = nn := heqSameLeftLen (congrArg (·+1) he₂) (Nat.succ_pos _) he₃
-      have : m = mm := heqSameRightLen (congrArg (·+1) he₂) (Nat.succ_pos _) he₃
-      subst nn mm
-      simp only [heq_eq_eq, branch.injEq] at he₃
-      -- yeah, no more HEq fuglyness!
-      have : v = vv := he₃.left
-      have : l = ll := he₃.right.left
-      have : r = rr := he₃.right.right
-      subst vv ll rr
-      split at he₁
-      <;> rename_i goLeft
-      <;> simp only [goLeft, and_self, ↓reduceDIte, Fin.isValue]
-      case' isTrue =>
-        cases l;
-        case leaf => exact absurd goLeft.left $ Nat.not_lt_zero m
-        rename_i o p _ _ _ _ _ _ _
-      case' isFalse =>
-        cases r;
-        case leaf => simp (config := { ground := true }) only [and_true, Nat.not_lt, Nat.le_zero_eq] at goLeft;
-                     exact absurd ((Nat.add_zero n).substr goLeft.symm) n_m_not_zero
-      all_goals
-        have he₁ := Fin.val_eq_of_eq he₁
-        simp only [Fin.isValue, Fin.val_succ, Fin.coe_castLE, Fin.coe_addNat, Nat.reduceEqDiff] at he₁
-        have : max_height_difference_2 = max_height_difference := rfl
-        have : subtree_full2 = subtree_full := rfl
-        subst max_height_difference_2 subtree_full2
-        rename_i del1 del2
-        clear del1 del2
-      case' isTrue =>
-        have : j < o + p + 1 := by omega --from he₁. It has j = (blah : Fin (o+p+1)).val
-      case' isFalse =>
-        have : ¬j<n := by omega --from he₁. It has j = something + n.
-      all_goals
-        simp only [this, ↓reduceDIte, Nat.pred_succ, Fin.isValue]
-        subst j -- overkill, but unlike rw it works
-        simp only [Nat.pred_succ, Fin.isValue, Nat.add_sub_cancel, Fin.eta]
+    case isTrue goLeft =>
+      match _term : n, l, m_le_n, max_height_difference, subtree_full with
+      | (nn+1), l ,m_le_n, max_height_difference, subtree_full =>
+      dsimp only [Fin.isValue, Nat.succ_eq_add_one]
+      rw[get_left, left_unfold]
+      case h₂ => exact Nat.succ_pos _
+      case h₃ => exact (Internal.heapRemoveLastAux (β := λ n ↦ α × Fin n) l _ _ _).2.snd.isLt
+      apply AdditionalProofs.heapRemoveLastWithIndexReturnsItemAtIndex
+    case isFalse goRight =>
+      dsimp only [Nat.pred_eq_sub_one, Nat.succ_eq_add_one, Fin.isValue]
+      cases r -- to work around cast
+      case leaf => simp (config:={ground:=true}) at goRight; exact absurd goRight.symm n_m_not_zero
+      case branch rv rl rr rm_le_n rmax_height_difference rsubtree_full =>
+        rw[get_right, right_unfold]
+        case h₂ => simp_arith[leftLen_unfold]
+        simp only [Fin.isValue, Fin.val_succ, Fin.coe_castLE, Fin.coe_addNat, leftLen_unfold]
+        have : ∀(a : Nat), a + n + 1 - n - 1 = a := λa↦(Nat.add_sub_cancel _ _).subst $ (Nat.add_assoc a n 1).subst (motive := λx↦a+n+1-n-1 = x-(n+1)) $ (Nat.sub_sub (a+n+1) n 1).subst rfl
+        simp only[this]
         apply AdditionalProofs.heapRemoveLastWithIndexReturnsItemAtIndex
-        done
+
 
 protected theorem heapRemoveLastWithIndexLeavesRoot {α : Type u} {n: Nat} (heap : CompleteTree α (n+1)) (h₁ : n > 0) : heap.root (Nat.succ_pos n) = (CompleteTree.Internal.heapRemoveLastWithIndex heap).fst.root h₁ :=
   CompleteTree.heapRemoveLastAuxLeavesRoot heap _ _ _ h₁
@@ -267,7 +222,6 @@ if h₃ : p < o ∧ (p + 1).nextPowerOfTwo = p + 1 then
         rewrite[←lens_see_through_cast _ leftLen _ (Nat.succ_pos _) _]
         rewrite[leftLen_unfold]
         assumption
-        omega
       simp only [Nat.add_eq, ne_eq, Fin.zero_eta, Nat.succ_eq_add_one, Nat.pred_eq_sub_one,
         Fin.coe_pred, Fin.isValue, ← lens_see_through_cast _ leftLen _ (Nat.succ_pos _) _]
       simp only[leftLen_unfold]
@@ -502,10 +456,10 @@ protected theorem heapRemoveLastWithIndexEitherContainsOrReturnsElement {α : Ty
   else by
     right
     have h₂ := CompleteTree.AdditionalProofs.heapRemoveLastWithIndexReturnsItemAtIndex heap
-    unfold get
     simp at h₁
     subst index
-    exact h₂.symm
+    rw[h₂]
+    rfl
 
 /--
   Shows that each element contained before removing the last that is not the last is still contained after removing the last.
